real world syntax

RealWorld.v
@@ -25,35 +25,27 @@ Record symmetric_key :=
 Record asymmetric_key :=
   {a_key_id : nat ;
    a_generator_id : user_id ;
-   a_usage : asymmetric_usage}.
+   a_usage : asymmetric_usage ;
+   a_paired_key_id : nat}.
 
 Inductive key :=
 | SKey (k : symmetric_key)
-| Akey (k : asymmetric_key).
+| AKey (k : asymmetric_key).
 
-(* POC type of ciphertypes *)
-Inductive ciphertype := 
-| type : ciphertype
-| type' : ciphertype
-| type'' : ciphertype.
-
+(* Changing (k : key) to (k_id : nat) in Ciphertext.
+ * When a user will decrypt a ciphertext, it will provide a key var.
+ *  That key var should map to a key, which has the same key_id that
+ *  matches the one necessary for the ciphertext.
+ *
+ * This change may also need to be done on Signature and HMAC message
+ *)
 Inductive message :=
 | Plaintext (txt : string)
-| Ciphertext (msg : message) (cipher : ciphertype) (k : key)
+| Ciphertext (msg : message) (k_id : nat)
 | Key_message (k : key)
-| Signature (k : asymmetric_key) (signer_id : user_id) (msg : message)
+| Signature (k_id : nat) (signer_id : user_id) (msg : message)
 | HMAC_message (k : symmetric_key) (msg : message).
 
-Record user :=
-  {uid : user_id ;
-   key_heap : fmap var key ;
-   mem_heap : fmap var message ;
-   protocol : list var ;
-   is_admin : bool }.
-
-(* POC newtork_message. Used for modeling
- * the network
- *)
 Inductive network_message :=
 | nmessage (msg : message) (uid : user_id).
 
@@ -66,24 +58,250 @@ Inductive user_cmd :=
 | Encrypt (k : key) (ptxt : message)
 | Sign (k : key) (msg : message)
 | Verify (k : key) (sig : message)
+| ProduceHMAC (k : key) (msg : message)
+| VerifyHMAC (k : key) (mac : message)
+| BindSKey (c1 : user_cmd) (c2 : key -> user_cmd)
+| BindAKeys (c1 : user_cmd) (c2 : (key * key) -> user_cmd)
+| GenerateSKey (usage : symmetric_usage)
+| GenerateAKeys (usage : asymmetric_usage)
 | Barrier.
 
-Notation "x <- c1 ; c2" := (Bind c1 (fun x => c2)) (right associativity, at level 75).
+Record user_data :=
+  {uid : user_id ;
+   key_heap : fmap var key ;
+   mem_heap : fmap var message ;
+   protocol : user_cmd ;
+   is_admin : bool }.
 
-(* 
-Work in Progress
- *)
+Notation "x <- c1 ; c2" := (Bind c1 (fun x => c2)) (right associativity, at level 75).
+Notation "x <<- c1 ; c2" := (BindSKey c1 (fun x => c2)) (right associativity, at level 75).
+Notation "x >--- c1 ; c2" := (BindAKeys c1 (fun x => c2)) (right associativity, at level 75).
+
 Record network := construct_network
-  { users : fmap user_id (list message) ;
+  { users_msg_buffer : fmap user_id (list message) ;
     trace : list (user_id * message) }.
 
+(* Hack to keep track of key_ids : key_counter *)
+Record universe := construct_universe
+  { users : fmap user_id user_data ;
+    net : network ;
+    key_counter : nat }.
 
-Inductive step : network -> network -> Prop :=
-| 
+(* For the below, the cmd's will be removed from protocol in the step function to 
+ * resemble what is done in the ideal model 
+ *)
+Definition send_message (msg_var : var) (from_user to_user : user_id) (U : universe) :=
+match U.(users) $? from_user with
+| Some u_data => match u_data.(mem_heap) $? msg_var with
+                 | Some msg => match (U.(net)).(users_msg_buffer) $? to_user with
+                               | Some msg_lst => {| users := U.(users) ;
+                                                    net := {| users_msg_buffer := (U.(net)).(users_msg_buffer) $+ (to_user, msg_lst ++ [msg]) ;
+                                                              trace := (to_user , msg) :: (U.(net)).(trace) |} ;
+                                                    key_counter := U.(key_counter) |}
+                               | None => U
+                               end
+                 | _ => U (* There was no matching msg to the var *)
+                 end
+| _ => U (* The sender is not valid *)
+end.
+
+Definition generate_symmetric_key (generator : user_id) (key_var : var) (U : universe) (usage : symmetric_usage) :=
+match U.(users) $? generator with
+| Some u_data => {| users := U.(users) $+ (generator, {| uid := generator ;
+                                                         key_heap := u_data.(key_heap) $+ (key_var, SKey {| s_key_id := U.(key_counter) ;
+                                                                                                            s_generator_id := generator ;
+                                                                                                            s_usage := usage |}) ;
+                                                         mem_heap := u_data.(mem_heap) ;
+                                                         protocol := u_data.(protocol) ;
+                                                         is_admin := u_data.(is_admin) |}) ;
+                    net := U.(net) ;
+                    key_counter := U.(key_counter) + 1 |}
+| None => U
+end.
+
+Definition generate_asymmetric_key (generator : user_id) (key_var1 key_var2 : var) (U : universe) (usage : asymmetric_usage) :=
+let usage' := match usage with
+              | RSA_E => RSA_D
+              | RSA_D => RSA_E
+              | ECDSA_S => ECDSA_V
+              | ECDSA_V => ECDSA_S
+              end in
+match U.(users) $? generator with
+| Some u_data => {| users := U.(users) $+ (generator, {| uid := generator ;
+                                                         key_heap := u_data.(key_heap) $+ (key_var1, AKey {| a_key_id := U.(key_counter) ;
+                                                                                                             a_generator_id := generator ;
+                                                                                                             a_usage := usage ;
+                                                                                                             a_paired_key_id := U.(key_counter) + 1 |})
+                                                                                       $+ (key_var2, AKey {| a_key_id := U.(key_counter) + 1 ;
+                                                                                                             a_generator_id := generator ;
+                                                                                                             a_usage := usage' ;
+                                                                                                             a_paired_key_id := U.(key_counter) |}) ;
+                                                         mem_heap := u_data.(mem_heap) ;
+                                                         protocol := u_data.(protocol) ;
+                                                         is_admin := u_data.(is_admin) |}) ;
+                    net := U.(net) ;
+                    key_counter := U.(key_counter) + 2 |}
+| None => U
+end.
+
+Definition recv_message (reading_user : user_id) (U : universe) (x : var) :=
+match (U.(net)).(users_msg_buffer) $? reading_user with
+| Some msg_lst => match msg_lst with
+                  | [] => U
+                  | h::t => match U.(users) $? reading_user with 
+                            | Some u_data => match h with
+                                             | Key_message k => {| users := U.(users) $+
+                                                                            (reading_user , {| uid := u_data.(uid) ;
+                                                                                               key_heap := u_data.(key_heap) $+ (x, k) ;
+                                                                                               mem_heap := u_data.(mem_heap) ;
+                                                                                               protocol := u_data.(protocol) ;
+                                                                                               is_admin := u_data.(is_admin) |}) ;
+                                                                   net := {| users_msg_buffer := (U.(net)).(users_msg_buffer) $+ (reading_user, t) ;
+                                                                             trace := (U.(net)).(trace) |} ;
+                                                                   key_counter := U.(key_counter) |}
+                                             | _ => {| users := U.(users) $+ (reading_user , {| uid := u_data.(uid) ;
+                                                                                                key_heap := u_data.(key_heap) ;
+                                                                                                mem_heap := u_data.(mem_heap) $+ (x, h) ;
+                                                                                                protocol := u_data.(protocol) ;
+                                                                                                is_admin := u_data.(is_admin) |}) ;
+                                                       net := {| users_msg_buffer := (U.(net)).(users_msg_buffer) $+ (reading_user, t) ;
+                                                                 trace := (U.(net)).(trace) |} ;
+                                                       key_counter := U.(key_counter) |}
+                                             end
+                            | None => U
+                            end
+                  end
+| None => U
+end.
+
+(* Changed decrypt_message to change on key_id of symmetric or asymmetric key instead of the key itself *)
+Definition decrypt_message (u_id : user_id) (msg_var msg_var': var) (U : universe) (key_var : var) :=
+match U.(users) $? u_id with
+| Some u_data => match u_data.(mem_heap) $? msg_var with
+                 | Some msg => match u_data.(key_heap) $? key_var with
+                               | Some (SKey k) => match msg with
+                                                  | Ciphertext msg' k' => match k.(s_key_id) with
+                                                                                 | k' => match msg' with
+                                                                                         | Key_message km => {| users := U.(users) $+ (u_id , {| uid := u_id ;
+                                                                                                                                                 key_heap := u_data.(key_heap) $+ (msg_var', km) ;
+                                                                                                                                                 mem_heap := u_data.(mem_heap) ;
+                                                                                                                                                 protocol := u_data.(protocol) ;
+                                                                                                                                                 is_admin := u_data.(is_admin) |}) ;
+                                                                                                                net := U.(net) ;
+                                                                                                                key_counter := U.(key_counter) |}
+                                                                                         | _ => {| users := U.(users) $+ (u_id , {| uid := u_id ;
+                                                                                                                                    key_heap := u_data.(key_heap) ;
+                                                                                                                                    mem_heap := u_data.(mem_heap) $+ (msg_var', msg') ;
+                                                                                                                                    protocol := u_data.(protocol) ;
+                                                                                                                                    is_admin := u_data.(is_admin) |}) ;
+                                                                                                   net := U.(net) ;
+                                                                                                   key_counter := U.(key_counter) |}
+                                                                                         end
+                                                                                 end
+                                                  | _ => U (* There was nothing to decrypt *)
+                                                  end
+                               | Some (AKey k) => match msg with
+                                                  | Ciphertext msg' k' => match k.(a_key_id) with 
+                                                                                 | k' => match msg' with
+                                                                                         | Key_message km => {| users := U.(users) $+ (u_id , {| uid := u_id ;
+                                                                                                                                                 key_heap := u_data.(key_heap) $+ (msg_var', km) ;
+                                                                                                                                                 mem_heap := u_data.(mem_heap) ;
+                                                                                                                                                 protocol := u_data.(protocol) ;
+                                                                                                                                                 is_admin := u_data.(is_admin) |}) ;
+                                                                                                                net := U.(net) ;
+                                                                                                                key_counter := U.(key_counter) |}
+                                                                                         | _ => {| users := U.(users) $+ (u_id , {| uid := u_id ;
+                                                                                                                                    key_heap := u_data.(key_heap) ;
+                                                                                                                                    mem_heap := u_data.(mem_heap) $+ (msg_var', msg') ;
+                                                                                                                                    protocol := u_data.(protocol) ;
+                                                                                                                                    is_admin := u_data.(is_admin) |}) ;
+                                                                                                   net := U.(net) ;
+                                                                                                   key_counter := U.(key_counter) |}
+                                                                                         end
+                                                                                 end
+                                                  | _ => U (* There was nothing to decrypt *)
+                                                  end
+                               | None => U (* Key_var does not correspond to a key *)
+                               end
+                 | None => U
+                 end
+| None => U
+end.
+
+(* Returns OPTION type *)
+Definition encrypt_message (u_id : user_id) (msg_var : var) (key_var : var) (U : universe) :=
+match U.(users) $? u_id with
+| Some u_data => match u_data.(mem_heap) $? msg_var with
+                 | Some msg => match u_data.(key_heap) $? key_var with
+                               | Some (AKey k) => match k.(a_usage) with
+                                                  | RSA_E => Some (Ciphertext msg k.(a_paired_key_id))
+                                                  | _ => None
+                                                  end
+                               | Some (SKey k') => match k'.(s_usage) with
+                                                   | HMAC => None
+                                                   | _ => Some (Ciphertext msg k'.(s_key_id))
+                                                   end
+                               | None => None
+                               end
+                 | None => None
+                 end
+| None => None
+end.
+
+(* Instead of signing a hash/message and appending to original message, the below
+ *  just signs and returns the message for now. Should work for our current purposes.
+ * The sign/verify also return an Option type for a message instead of editing the universe, i.e.,
+ *  adding messages to the memory heaps. Does this need to change? !!!!!!!!!!!
+ *)
+Definition sign (signee : user_id) (key_var msg_var signed_msg_var : var) (U : universe) :=
+match U.(users) $? signee with
+| Some u_data => match u_data.(mem_heap) $? msg_var with
+                 | Some msg => match u_data.(key_heap) $? key_var with
+                               | Some (AKey k) => match k.(a_usage) with
+                                                  | ECDSA_S => Some (Signature k.(a_paired_key_id) signee msg)
+                                                  | _ => None
+                                                  end
+                               | Some (SKey k') => None
+                               | _ => None
+                               end
+                 | None => None
+                 end
+| None => None
+end.
+
+Definition verify (verifier : user_id) (key_var signed_msg_var verified_msg_var : var) (U : universe) :=
+match U.(users) $? verifier with
+| Some u_data => match u_data.(mem_heap) $? signed_msg_var with
+                 | Some s_msg => match u_data.(key_heap) $? key_var with
+                                 | Some (AKey k) => match s_msg with
+                                                    | Signature k_id signee msg => if k_id =? k.(a_paired_key_id)
+                                                                                   then Some msg
+                                                                                   else None
+                                                    | _ => None
+                                                    end
+                                 | Some (SKey k') => None
+                                 | None => None
+                                 end
+                 | None => None
+                 end
+| None => None
+end.
 
 
+(* Ping Protocol *)
 
-
+  (* U.(users) *)
+Example ping_users :=
+ $0 $+ (0, {| uid := 0 ;
+              key_heap := $0 ;
+              mem_heap := $0 ;
+              protocol := (a >--- (GenerateAKeys RSA_E) ; (b <- (Send 1 (Key_message (match a with | (pair p s) => p end))) ; (c <<- (GenerateAKeys ECDSA_S) ; (d <- (Send 1 (Key_message c)) ; (e <- (Sign c (Plaintext "Hello")) ; (f <- (Encrypt (match a with | (pair p s) => p end) e) ; (g <- (Send 1 f) ; Recv))))))) ;
+              is_admin := false |})
+    $+ (1 , {| uid := 1 ;
+               key_heap := $0 ;
+               mem_heap := $0 ;
+               protocol := Barrier ;
+               is_admin := false |}).
 
 
 
